WIP

code/ecdsa/Hacl.Impl.EC.ScalarMult.Radix.fst
@@ -204,52 +204,56 @@ let not_equal_precomputed1 #c a b p0 =
 val not_equal_precomputed: #c: curve 
   -> z: nat
   -> p: Spec.ECC.point #c #Jacobian
+  -> p0: Spec.ECC.point #c #Jacobian 
   -> si: nat {si <= 16} -> Lemma
-    (requires ((z <= getOrder #c / 16) /\ pointEqual p (point_mult #c z (basePoint #c))))
+    (requires ((z <= getOrder #c / 16) /\ pointEqual p (point_mult #c z p0)))
     (ensures (
       let p_16 = Spec.ECC.Radix.getPointDoubleNTimes #c p 4 in 
-      ~ (pointEqual #c p_16 (point_mult #c si (basePoint #c))) \/ (
-      isPointAtInfinity #c #Jacobian p_16 /\ isPointAtInfinity #c #Jacobian (point_mult #c si (basePoint #c)))))
+      ~ (pointEqual #c p_16 (point_mult #c si p0)) \/ (
+      isPointAtInfinity #c #Jacobian p_16 /\ isPointAtInfinity #c #Jacobian (point_mult #c si p0))))
 
-let not_equal_precomputed #c z p si = 
-  point_mult_mult #c z 16 (basePoint #c);
-  not_equal_precomputed0 16 (point_mult z (basePoint #c)) p;
-  not_equal_precomputed1 #c si (16 * z) (basePoint #c)
+let not_equal_precomputed #c z p p0 si = 
+  point_mult_mult #c z 16 p0;
+  not_equal_precomputed0 16 (point_mult z p0) p;
+  not_equal_precomputed1 #c si (16 * z) p0
 
 
 val get_exists_: #c: curve
+  -> p0: Spec.ECC.point #c #Jacobian 
   -> p: Spec.ECC.point #c #Jacobian 
-    {exists (z: nat). ((z <= getOrder #c / 16) /\ pointEqual p (point_mult #c z (basePoint #c)))}
+    {exists (z: nat). ((z <= getOrder #c / 16) /\ pointEqual p (point_mult #c z p0))}
   -> z_test: nat {forall (z: nat {z < z_test}).
-    ~  ((z <= getOrder #c / 16) /\ pointEqual p (point_mult #c z (basePoint #c)))}
-  -> Tot (z: nat { (z <= getOrder #c / 16) /\ pointEqual p (point_mult #c z (basePoint #c))})
+    ~  ((z <= getOrder #c / 16) /\ pointEqual p (point_mult #c z p0))}
+  -> Tot (z: nat { (z <= getOrder #c / 16) /\ pointEqual p (point_mult #c z p0)})
   (decreases (getOrder #c - z_test))
 
-let rec get_exists_ #c p z = 
-  if (z <= getOrder #c / 16) && pointEqual p (point_mult #c z (basePoint #c)) 
+let rec get_exists_ #c p0 p z = 
+  if (z <= getOrder #c / 16) && pointEqual p (point_mult #c z p0) 
   then z
-  else get_exists_ #c p (z + 1)
+  else get_exists_ #c p0 p (z + 1)
 
 
 val get_exists: #c: curve
+  -> p0: Spec.ECC.point #c #Jacobian 
   -> p: Spec.ECC.point #c #Jacobian 
-    {exists (z: nat). ((z <= getOrder #c / 16) /\ pointEqual p (point_mult #c z (basePoint #c)))}
-  -> Tot (z: nat { ((z <= getOrder #c / 16) /\ pointEqual p (point_mult #c z (basePoint #c)))})
+    {exists (z: nat). ((z <= getOrder #c / 16) /\ pointEqual p (point_mult #c z p0))}
+  -> Tot (z: nat { ((z <= getOrder #c / 16) /\ pointEqual p (point_mult #c z p0))})
 
-let get_exists #c p = get_exists_ #c p 0
+let get_exists #c p0 p = get_exists_ #c p0 p 0
 
 
 val not_equal_precomputed2: #c: curve 
+  -> p0: Spec.ECC.point #c #Jacobian
   -> p: Spec.ECC.point #c #Jacobian
-       { exists (z: nat {z <= getOrder #c / 16}). pointEqual p (point_mult #c z (basePoint #c))}
+       { exists (z: nat {z <= getOrder #c / 16}). pointEqual p (point_mult #c z p0)}
   -> si: nat {si <= 16} -> Lemma (
     let p_16 = Spec.ECC.Radix.getPointDoubleNTimes #c p 4 in 
-    ~ (pointEqual #c p_16 (point_mult #c si (basePoint #c))) \/ (
-    isPointAtInfinity #c #Jacobian p_16 /\ isPointAtInfinity #c #Jacobian (point_mult #c si (basePoint #c))))
+    ~ (pointEqual #c p_16 (point_mult #c si p0)) \/ (
+    isPointAtInfinity #c #Jacobian p_16 /\ isPointAtInfinity #c #Jacobian (point_mult #c si p0)))
 
-let not_equal_precomputed2 #c p si = 
-  let z = get_exists #c p in 
-  not_equal_precomputed #c z p si
+let not_equal_precomputed2 #c p0 p si = 
+  let z = get_exists #c p0 p in 
+  not_equal_precomputed #c z p p0 si
   
   
 val radix_step_precomputed0: #c: curve -> p: Spec.ECC.point #c #Jacobian {isPointAtInfinity #c p} -> 
@@ -313,7 +317,7 @@ let radix_step_precomputed #c p tempBuffer scalar i =
 
     curve_compatibility_with_translation_lemma_1  (fromDomainPoint #c #DH (toJacobianCoordinates #c (point_affine_as_nat c h1 pointToAdd))) (point_mult #c si (basePoint #c)) pRadixed;
 
-    not_equal_precomputed2 #c (fromDomainPoint #c #DH (point_as_nat c h0 p)) si;
+    not_equal_precomputed2 #c (basePoint #c) (fromDomainPoint #c #DH (point_as_nat c h0 p)) si;
 
     if (isPointAtInfinity #c #Jacobian pRadixed && isPointAtInfinity #c #Jacobian pointPrecomputed) then 
 	radix_step_precomputed0 #c pRadixed
@@ -423,13 +427,13 @@ let montgomery_ladder_2_precomputed #c #a p scalar tempBuffer =
 	Spec.ECC.Radix.pred0 #c #Affine (fromDomainPoint #c #DH (point_as_nat c h0_ p)) (as_seq h0_ scalar) (basePoint #c) (v i - 1))
 
 
-let getPointTable (c: curve) (precomputedTable: lbuffer uint64 (getPointLen c *! 16ul)) (i: nat {i < 16}) : GTot (point c) = 
-  gsub precomputedTable (getPointLenU64 c *! size i) (getPointLenU64 c)
+let getPointTable (c: curve) (precomputedTable: lbuffer uint64 (getPointLenU64 c *! 16ul)) (i: nat {i < 16}) : GTot (point c) = 
+  gsub precomputedTable (size i *! getPointLenU64 c) (getPointLenU64 c)
 
 
 
 val getPointPrecomputedTable_: #c: curve -> k: size_t {v k < 16}
-  -> precomputedTable: lbuffer uint64 (getPointLen c *! 16ul)
+  -> precomputedTable: lbuffer uint64 (getPointLenU64 c *! 16ul)
   -> bits: uint64
   -> r: point c ->
   Stack unit 
@@ -437,13 +441,14 @@ val getPointPrecomputedTable_: #c: curve -> k: size_t {v k < 16}
     point_eval c h r /\ (
     forall (i: nat {i < 16}). let pi = getPointTable c precomputedTable i in point_eval c h pi) /\ (
     forall (i: nat {i < 16}). 
-      let pi = point_as_nat c h (getPointTable c precomputedTable i) in 
-      let p0 = point_as_nat c h (getPointTable c precomputedTable 0) in 
+      let pi = fromDomainPoint #c #DH (point_as_nat c h (getPointTable c precomputedTable i)) in 
+      let p0 = fromDomainPoint #c #DH (point_as_nat c h (getPointTable c precomputedTable 1)) in 
       pointEqual pi (point_mult #c i p0)))
   (ensures fun h0 _ h1 -> modifies (loc r) h0 h1 /\ point_eval c h1 r /\ (
-    let p0 = point_as_nat c h0 (getPointTable c precomputedTable 0) in 
+    let p0 = fromDomainPoint #c #DH (point_as_nat c h0 (getPointTable c precomputedTable 1)) in 
+    let pi = fromDomainPoint #c #DH (point_as_nat c h1 r) in 
     if v bits = v k then 
-      pointEqual (point_as_nat c h1 r) ((point_mult #c (v k) p0))
+      pointEqual pi (point_mult #c (v k) p0)
     else 
       point_as_nat c h1 r == point_as_nat c h0 r))
 
@@ -467,17 +472,16 @@ let getPointPrecomputedTable_ #c k precomputedTable bits r =
   let rZ = sub r (size 2 *! coordLen) coordLen in 
 
   let h1 = ST.get() in 
-
-  assert(let pi = getPointTable c precomputedTable (v k) in point_eval c h0 pi);
-  assert(let pi = gsub precomputedTable pointLen (getPointLenU64 c) in point_eval c h0 pi); 
   
   copy_conditional #c rX lut_cmb_x mask;
   copy_conditional #c rY lut_cmb_y mask;
   copy_conditional #c rZ lut_cmb_z mask
+  
 
 val lemma_test3__: #c: curve -> p: point c -> r: point c -> h0: mem 
   -> h1: mem {live h0 p /\ live h0 r /\ modifies (loc r) h0 h1 /\ disjoint p r /\ point_eval c h0 p} -> 
-  Lemma (point_eval c h1 p /\ point_as_nat c h0 p == point_as_nat c h1 p)
+  Lemma (point_eval c h1 p /\ point_as_nat c h0 p == point_as_nat c h1 p /\ 
+    fromDomainPoint #c #DH (point_as_nat c h0 p) == fromDomainPoint #c #DH (point_as_nat c h1 p))
 
 let lemma_test3__ #c p r h0 h1 = 
   assert(as_nat c h0 (gsub p (size 0) (getCoordinateLenU64 c)) == as_nat c h1 (gsub p (size 0) (getCoordinateLenU64 c)));
@@ -485,12 +489,13 @@ let lemma_test3__ #c p r h0 h1 =
   assert(as_nat c h0 (gsub p (2ul *! getCoordinateLenU64 c) (getCoordinateLenU64 c)) == as_nat c h1 (gsub p (2ul *! getCoordinateLenU64 c) (getCoordinateLenU64 c)))
 
 
-val lemma_test3_0: #c: curve -> precomputedTable: lbuffer uint64 (getPointLen c *! 16ul) 
+val lemma_test3_0: #c: curve -> precomputedTable: lbuffer uint64 (getPointLenU64 c *! 16ul) 
   -> h0: mem -> h1: mem -> i: nat {i < 16} -> r: point c -> Lemma
   (requires (live h0 precomputedTable /\ live h0 r /\ modifies (loc r) h0 h1 /\ disjoint precomputedTable r /\ (
     let pi = getPointTable c precomputedTable i in point_eval c h0 pi)))
   (ensures (
-   let pi = getPointTable c precomputedTable i in point_eval c h1 pi /\ point_as_nat c h0 pi == point_as_nat c h1 pi))
+   let pi = getPointTable c precomputedTable i in point_eval c h1 pi /\ point_as_nat c h0 pi == point_as_nat c h1 pi /\
+   fromDomainPoint #c #DH (point_as_nat c h0 pi) == fromDomainPoint #c #DH (point_as_nat c h1 pi)))
 
 let lemma_test3_0 #c precomputedTable h0 h1 i r = 
   let p = getPointTable c precomputedTable i in 
@@ -499,47 +504,73 @@ let lemma_test3_0 #c precomputedTable h0 h1 i r =
   lemma_test3__ #c p r h0 h1
 
 
-val lemma_test3_1: #c: curve -> precomputedTable: lbuffer uint64 (getPointLen c *! 16ul) 
+val lemma_test3_1: #c: curve -> precomputedTable: lbuffer uint64 (getPointLenU64 c *! 16ul) 
   -> h0: mem -> h1: mem ->  r: point c -> i: nat {i < 16} -> Lemma
   (requires (live h0 precomputedTable /\ live h0 r /\ modifies (loc r) h0 h1 /\ disjoint precomputedTable r /\ (
     let pi = getPointTable c precomputedTable i in
-    let p0 = getPointTable c precomputedTable 0 in 
-    point_eval c h0 pi /\ point_eval c h0 p0 /\ pointEqual (point_as_nat c h0 pi) (point_mult #c i (point_as_nat c h0 p0)))))
+    let p0 = getPointTable c precomputedTable 1 in 
+    point_eval c h0 pi /\ point_eval c h0 p0 /\ 
+    pointEqual (fromDomainPoint #c #DH (point_as_nat c h0 pi)) (point_mult #c i (fromDomainPoint #c #DH (point_as_nat c h0 p0))))))
   (ensures (
     let pi = getPointTable c precomputedTable i in 
-    let p0 = getPointTable c precomputedTable 0 in 
-    point_eval c h1 pi /\ point_eval c h1 p0 /\ pointEqual (point_as_nat c h1 pi) (point_mult #c i (point_as_nat c h1 p0))))
+    let p0 = getPointTable c precomputedTable 1 in 
+    point_eval c h1 pi /\ point_eval c h1 p0 /\ 
+    pointEqual (fromDomainPoint #c #DH (point_as_nat c h1 pi)) (point_mult #c i (fromDomainPoint #c #DH (point_as_nat c h1 p0)))))
 
 let lemma_test3_1 #c precomputedTable h0 h1 r i = 
   lemma_test3_0 #c precomputedTable h0 h1 i r;
-  lemma_test3_0 #c precomputedTable h0 h1 0 r
+  lemma_test3_0 #c precomputedTable h0 h1 1 r
   
 
-val lemma_test3: #c: curve -> precomputedTable: lbuffer uint64 (getPointLen c *! 16ul) 
+val lemma_test3: #c: curve -> precomputedTable: lbuffer uint64 (getPointLenU64 c *! 16ul) 
   -> h0: mem -> h1: mem -> r: point c -> Lemma
   (requires (live h0 precomputedTable /\ live h0 r /\ disjoint precomputedTable r /\ modifies (loc r) h0 h1 /\ 
     (forall (i: nat {i < 16}). 
       let pi = getPointTable c precomputedTable i in point_eval c h0 pi) /\
-    (forall (i: nat {i < 16}). let pi = point_as_nat c h0 (getPointTable c precomputedTable i) in 
-      let p0 = point_as_nat c h0 (getPointTable c precomputedTable 0) in pointEqual pi (point_mult #c i p0))))
+    (forall (i: nat {i < 16}). 
+      let pi = fromDomainPoint #c #DH (point_as_nat c h0 (getPointTable c precomputedTable i)) in 
+      let p0 = fromDomainPoint #c #DH (point_as_nat c h0 (getPointTable c precomputedTable 1)) in 
+      pointEqual pi (point_mult #c i p0))))
   (ensures (
     (forall (i: nat {i < 16}). let pi = getPointTable c precomputedTable i in point_eval c h1 pi) /\
-    (forall (i: nat {i < 16}). let pi = point_as_nat c h1 (getPointTable c precomputedTable i) in 
-      let p0 = point_as_nat c h1 (getPointTable c precomputedTable 0) in pointEqual pi (point_mult #c i p0))))
+    (forall (i: nat {i < 16}). 
+      let pi = fromDomainPoint #c #DH (point_as_nat c h1 (getPointTable c precomputedTable i)) in 
+      let p0 = fromDomainPoint #c #DH (point_as_nat c h1 (getPointTable c precomputedTable 1)) in 
+      pointEqual pi (point_mult #c i p0))))
+
+
+assume val lemma_test4: #c: curve -> precomputedTable: lbuffer uint64 (getPointLenU64 c *! 16ul) 
+  -> h0: mem -> h1: mem -> p: point c ->  Lemma
+  (requires (live h0 precomputedTable /\ modifies0 h0 h1 /\ point_eval c h0 p /\
+    (forall (i: nat {i < 16}). 
+      let pi = getPointTable c precomputedTable i in point_eval c h0 pi) /\
+    (forall (i: nat {i < 16}). 
+      let pi = fromDomainPoint #c #DH (point_as_nat c h0 (getPointTable c precomputedTable i)) in 
+      let p0 = fromDomainPoint #c #DH (point_as_nat c h0 (getPointTable c precomputedTable 1)) in 
+      pointEqual pi (point_mult #c i p0))))
+  (ensures (point_eval c h1 p /\ 
+    (forall (i: nat {i < 16}). let pi = getPointTable c precomputedTable i in point_eval c h1 pi) /\
+    (forall (i: nat {i < 16}). 
+      let pi = fromDomainPoint #c #DH (point_as_nat c h1 (getPointTable c precomputedTable i)) in 
+      let p0 = fromDomainPoint #c #DH (point_as_nat c h1 (getPointTable c precomputedTable 1)) in 
+      let p  = fromDomainPoint #c #DH (point_as_nat c h1 p) in 
+      pointEqual pi (point_mult #c i p0) /\ ~ (isPointAtInfinity #c p0) /\ (exists (z: nat {z <= getOrder #c / 16}). pointEqual p (point_mult #c z p0)))))
+      
 
 let lemma_test3 #c precomputedTable h0 h1 r = 
   let a : Type = (a: nat {a < 16}) in 
   let p : (a -> GTot Type)  = 
     fun i -> 
       let pi = getPointTable c precomputedTable i in 
-      let p0 = getPointTable c precomputedTable 0 in 
-      point_eval c h1 pi /\ point_eval c h1 p0 /\ pointEqual (point_as_nat c h1 pi) (point_mult #c i (point_as_nat c h1 p0)) in 
+      let p0 = getPointTable c precomputedTable 1 in 
+      point_eval c h1 pi /\ point_eval c h1 p0 /\ 
+      pointEqual (fromDomainPoint #c #DH (point_as_nat c h1 pi)) (point_mult #c i (fromDomainPoint #c #DH (point_as_nat c h1 p0))) in 
   let pred: (x : a -> Lemma (p x)) = lemma_test3_1 #c precomputedTable h0 h1 r in 
   Classical.forall_intro #a #_ pred
 
 
 val getPointPrecomputedTable_1: #c: curve 
-  -> precomputedTable: lbuffer uint64 (getPointLen c *! 16ul)
+  -> precomputedTable: lbuffer uint64 (getPointLenU64 c *! 16ul)
   -> bits: uint64 {v bits < 16}
   -> r: point c ->
   Stack unit 
@@ -547,146 +578,479 @@ val getPointPrecomputedTable_1: #c: curve
     point_eval c h r /\ (
     forall (i: nat {i < 16}). let pi = getPointTable c precomputedTable i in point_eval c h pi) /\ (
     forall (i: nat {i < 16}). 
-      let pi = point_as_nat c h (getPointTable c precomputedTable i) in 
-      let p0 = point_as_nat c h (getPointTable c precomputedTable 0) in 
-      pointEqual pi (point_mult #c i p0)))
+      let pi = fromDomainPoint #c #DH (point_as_nat c h (getPointTable c precomputedTable i)) in 
+      let p1 = fromDomainPoint #c #DH (point_as_nat c h (getPointTable c precomputedTable 1)) in 
+      pointEqual pi (point_mult #c i p1)))
   (ensures fun h0 _ h1 -> modifies (loc r) h0 h1 /\ point_eval c h1 r /\ (
-    let p0 = point_as_nat c h0 (getPointTable c precomputedTable 0) in 
-    pointEqual (point_as_nat c h1 r) (point_mult #c (v bits) p0)))
+    let p1 = getPointTable c precomputedTable 1 in 
+    let p1 = fromDomainPoint #c #DH (point_as_nat c h0 p1) in 
+    let rD = fromDomainPoint #c #DH (point_as_nat c h1 r) in 
+    pointEqual rD (point_mult #c (v bits) p1)))
 
 let getPointPrecomputedTable_1 #c precomputedTable bits r = 
   let h0 = ST.get() in 
   let inv (h: mem) (k: nat {0 <= k /\ k <= 16}) : Type0 = modifies (loc r) h0 h /\ point_eval c h r /\ 
     disjoint r precomputedTable /\ (
-    let p0 = getPointTable c precomputedTable 0 in 
+    let p0 = getPointTable c precomputedTable 1 in 
     (forall (i: nat {i < 16}). let pi = getPointTable c precomputedTable i in point_eval c h pi) /\
     (forall (i: nat {i < 16}). 
-      let pi = point_as_nat c h (getPointTable c precomputedTable i) in 
-      pointEqual pi (point_mult #c i (point_as_nat c h p0))) /\ (
+      let pi = fromDomainPoint #c #DH (point_as_nat c h (getPointTable c precomputedTable i)) in 
+      let p0 = fromDomainPoint #c #DH (point_as_nat c h p0) in 
+      pointEqual pi (point_mult #c i p0)) /\ (
     if v bits < k then 
-      pointEqual (point_as_nat c h r) (point_mult #c (v bits) (point_as_nat c h0 p0))
+      pointEqual (fromDomainPoint #c #DH (point_as_nat c h r)) (point_mult #c (v bits)
+	(fromDomainPoint #c #DH (point_as_nat c h0 p0)))
     else 
       point_as_nat c h r == point_as_nat c h0 r)) in 
 
   let f = fun (k: size_t {0 <= v k /\ v k < 16})  ->
-      let h0_ = ST.get() in 
-      getPointPrecomputedTable_ k precomputedTable bits r;
-      let h1 = ST.get() in
-      lemma_test3 #c precomputedTable h0 h1 r;
-
-      assert (modifies (loc r) h0 h0_);
-      lemma_test3__ (getPointTable c precomputedTable 0) r h0 h0_ in 
+    let h0_ = ST.get() in 
+    getPointPrecomputedTable_ k precomputedTable bits r; 
+    let h1 = ST.get() in
+    lemma_test3 #c precomputedTable h0 h1 r;
+    assert (modifies (loc r) h0 h0_);
+    lemma_test3__ (getPointTable c precomputedTable 1) r h0 h0_ in 
 
   Lib.Loops.for (size 0) (size 16) inv f
 
 
 val getPointPrecomputedTable: #c: curve -> #buf_type: buftype
   -> scalar: scalar_t #buf_type #c
-  -> precomputedTable: lbuffer uint64 (getPointLen c *! 16ul)
-  -> bits: uint64 {v bits < 16}
+  -> precomputedTable: lbuffer uint64 (getPointLenU64 c *! 16ul)
+  -> i: size_t {v i < v (getScalarLenBytes c) * 2}
   -> r: point c ->
   Stack unit 
-  (requires fun h -> live h precomputedTable /\ live h r /\ disjoint r precomputedTable /\
+  (requires fun h -> live h precomputedTable /\ live h r /\ live h scalar /\ disjoint r precomputedTable /\
     point_eval c h r /\ (
     forall (i: nat {i < 16}). let pi = getPointTable c precomputedTable i in point_eval c h pi) /\ (
     forall (i: nat {i < 16}). 
-      let pi = point_as_nat c h (getPointTable c precomputedTable i) in 
-      let p0 = point_as_nat c h (getPointTable c precomputedTable 0) in 
+      let pi = fromDomainPoint #c #DH (point_as_nat c h (getPointTable c precomputedTable i)) in 
+      let p0 = fromDomainPoint #c #DH (point_as_nat c h (getPointTable c precomputedTable 1)) in 
       pointEqual pi (point_mult #c i p0)))
   (ensures fun h0 _ h1 -> modifies (loc r) h0 h1 /\ point_eval c h1 r /\ (
-    let p0 = point_as_nat c h0 (getPointTable c precomputedTable 0) in 
-    pointEqual (point_as_nat c h1 r) (point_mult #c (v bits) p0)))
-
+    let p0 = fromDomainPoint #c #DH (point_as_nat c h0 (getPointTable c precomputedTable 1)) in 
+    let bits = Math.Lib.arithmetic_shift_right (scalar_as_nat #c (as_seq h0 scalar)) (v (getScalarLen c) - (v i + 1) * 4) % pow2 4 in 
+    pointEqual (fromDomainPoint #c #DH (point_as_nat c h1 r)) (point_mult #c bits p0) /\
+    pointEqual (fromDomainPoint #c #DH (point_as_nat c h1 r)) (Spec.ECC.Radix.getPrecomputedPoint #c #Jacobian p0 bits)))
 
 
 let getPointPrecomputedTable #c #buf_type scalar precomputedTable i pointToAdd = 
   let h0 = ST.get() in 
-    
   let bits = getScalar_4_byBit #c scalar i in 
+  let h1 = ST.get() in 
+
+  Hacl.Impl.P.PointAdd.Aux.lemma_coord_eval c h0 h1 pointToAdd;
+  lemma_test3 #c precomputedTable h0 h1 pointToAdd; 
+  getPointPrecomputedTable_1 precomputedTable bits pointToAdd; 
   
-  let invK (h: mem) (k: nat {0 <= k /\ k <= 16}) : Type0 = modifies (loc pointToAdd) h0 h in 
-  let f =  (fun (k: size_t {v k >= 0 /\ v k < 16}) -> 
-    admit(); 
-    getPointPrecomputedTable_ k precomputedTable bits pointToAdd;
-    admit()) in
+  lemma_test3__ (getPointTable c precomputedTable 1) pointToAdd h0 h1
+
+ 
+
+inline_for_extraction noextract  
+val montgomery_ladder_step_radix_0: #c: curve -> #buf_type: buftype
+  -> p: point c 
+  -> scalar: scalar_t #buf_type #c
+  -> precomputedTable: lbuffer uint64 (getPointLenU64 c *! 16ul)
+  -> i: size_t {v i < v (getScalarLenBytes c) * 2}
+  -> tempBuffer: lbuffer uint64 (size 17 *! getCoordinateLenU64 c) 
+  -> r: point c ->
+  Stack unit 
+  (requires fun h -> live h precomputedTable /\ live h r /\ live h tempBuffer /\  live h scalar /\ live h p /\
+    disjoint r precomputedTable /\ disjoint p r /\ disjoint r tempBuffer /\
+    point_eval c h r /\ disjoint p tempBuffer /\ point_eval c h p  /\ (
+    forall (i: nat {i < 16}). let pi = getPointTable c precomputedTable i in point_eval c h pi) /\ (
+    forall (i: nat {i < 16}). 
+      let pi = fromDomainPoint #c #DH (point_as_nat c h (getPointTable c precomputedTable i)) in 
+      let p1 = fromDomainPoint #c #DH (point_as_nat c h (getPointTable c precomputedTable 1)) in 
+      pointEqual pi (point_mult #c i p1)))
+  (ensures fun h0 _ h1 -> modifies (loc r |+| loc tempBuffer |+| loc p) h0 h1 /\ 
+    point_eval c h1 p /\ point_eval c h1 r /\ (
+    let p1 = fromDomainPoint #c #DH (point_as_nat c h0 (getPointTable c precomputedTable 1)) in 
+    let bits = Math.Lib.arithmetic_shift_right (scalar_as_nat #c (as_seq h0 scalar)) (v (getScalarLen c) - (v i + 1) * 4) % pow2 4 in 
+    pointEqual (fromDomainPoint #c #DH (point_as_nat c h1 r)) (Spec.ECC.Radix.getPrecomputedPoint #c #Jacobian p1 bits) /\   
+    fromDomainPoint #c #DH (point_as_nat c h1 p) == Spec.ECC.Radix.getPointDoubleNTimes #c (fromDomainPoint #c #DH (point_as_nat c h0 p)) 4))
+
+
+let montgomery_ladder_step_radix_0 #c #b p scalar precomputedTable i tempBuffer r = 
+    let h0 = ST.get() in 
+  getPointPrecomputedTable #c scalar precomputedTable i r;
+    let h1 = ST.get() in 
+    Hacl.Impl.P.PointAdd.Aux.lemma_coord_eval c h0 h1 p; 
+  getPointDoubleNTimes #c p tempBuffer; 
+    let h2 = ST.get() in 
+
+  Hacl.Impl.P.PointAdd.Aux.lemma_coord_eval c h0 h1 p;
+  Hacl.Impl.P.PointAdd.Aux.lemma_coord_eval c h1 h2 r
+
+
+val montgomery_ladder_step_radix_1_lemma: #c: curve -> scalar: scalar_bytes #c
+  -> p0: point_nat_prime #c {~ (isPointAtInfinity #c p0)} 
+  -> p: point_nat_prime #c {exists (z: nat {z <= getOrder #c / 16}). pointEqual p (point_mult #c z p0)} 
+  -> pi: point_nat_prime #c -> r: point_nat_prime #c 
+  -> i: nat {i >= 1 /\ i < v (getScalarLenBytes c) * 2} -> 
+   Lemma 
+     (requires (  
+       let scalar = scalar_as_nat scalar in 
+       let si = Math.Lib.arithmetic_shift_right scalar (v (getScalarLen c) - (i + 1) * 4) % pow2 4 in 
+       let pointRadixed =  Spec.ECC.Radix.getPointDoubleNTimes #c p 4 in 
+       pointEqual pi (Spec.ECC.Radix.getPrecomputedPoint #c #Jacobian p0 si) /\ r == _point_add #c pi pointRadixed))
+   (ensures (pointEqual #c r (Spec.ECC.Radix.radix_step #c #Jacobian scalar p0 (i - 1) p)))
+
+let montgomery_ladder_step_radix_1_lemma #c k p0 p pi r i = 
+  let scalar = scalar_as_nat k in 
+  let l = v (getScalarLen c) in 
+  let si = Math.Lib.arithmetic_shift_right scalar (l - ((i - 1) + 2) * 4) % pow2 4 in 
+  let pointRadixed = Spec.ECC.Radix.getPointDoubleNTimes #c p 4 in 
+  let pointPrecomputed = (Spec.ECC.Radix.getPrecomputedPoint #c #Jacobian p0 si) in 
+
+  not_equal_precomputed2 #c p0 p si;
+  curve_order_is_the_smallest #c p0;
+  curve_compatibility_with_translation_lemma pi pointPrecomputed pointRadixed; 
+  curve_commutativity_lemma pointPrecomputed pointRadixed
+
+
+
+inline_for_extraction noextract  
+val montgomery_ladder_step_radix: #c: curve -> #buf_type: buftype
+  -> p: point c 
+  -> scalar: scalar_t #buf_type #c
+  -> precomputedTable: lbuffer uint64 (getPointLenU64 c *! 16ul)
+  -> i: size_t {v i >= 1 /\ v i < v (getScalarLenBytes c) * 2}
+  -> tempBuffer: lbuffer uint64 (size 17 *! getCoordinateLenU64 c) 
+  -> r: point c ->
+  Stack unit 
+  (requires fun h -> live h precomputedTable /\ live h r /\ live h tempBuffer /\  live h scalar /\ live h p /\
+    disjoint r precomputedTable /\ disjoint p r /\ disjoint r tempBuffer /\
+    point_eval c h r /\ disjoint p tempBuffer /\ point_eval c h p  /\ (
+    forall (i: nat {i < 16}). let pi = getPointTable c precomputedTable i in point_eval c h pi) /\ (
+    forall (i: nat {i < 16}). 
+      let pi = fromDomainPoint #c #DH (point_as_nat c h (getPointTable c precomputedTable i)) in 
+      let p1 = fromDomainPoint #c #DH (point_as_nat c h (getPointTable c precomputedTable 1)) in 
+      let p  = fromDomainPoint #c #DH (point_as_nat c h p) in 
+      ~ (isPointAtInfinity #c p1) /\
+	(exists (z: nat {z <= getOrder #c / 16}). pointEqual p (point_mult #c z p1)) /\ pointEqual pi (point_mult #c i p1)))
+  (ensures fun h0 _ h1 -> modifies (loc r |+| loc tempBuffer |+| loc p) h0 h1 /\ point_eval c h1 p /\ (
+    let p1 = fromDomainPoint #c #DH (point_as_nat c h0 (getPointTable c precomputedTable 1)) in 
+    let r =  fromDomainPoint #c #DH (point_as_nat c h1 p) in 
+    let p = (fromDomainPoint #c #DH (point_as_nat c h0 p)) in 
+    pointEqual #c r (Spec.ECC.Radix.radix_step #c #Jacobian (as_seq h0 scalar) p1 (v i - 1) p)))
+
+
+let montgomery_ladder_step_radix #c #b p scalar table i tempBuffer r = 
+  let h0 = ST.get() in 
+  montgomery_ladder_step_radix_0 p scalar table i tempBuffer r;
+  let h1 = ST.get() in 
+  point_add r p p tempBuffer;
+
+  let h2 = ST.get() in 
+  
+  let p1 = fromDomainPoint #c #DH (point_as_nat c h0 (getPointTable c table 1)) in 
+  let pi = (fromDomainPoint #c #DH (point_as_nat c h1 r)) in 
+  let r =  fromDomainPoint #c #DH (point_as_nat c h2 p) in 
+  let p = (fromDomainPoint #c #DH (point_as_nat c h0 p)) in 
+
+  montgomery_ladder_step_radix_1_lemma #c (as_seq h0 scalar) p1 p pi r (v i)
+
+
+val lemma_pointAtInfInDomain1: #c: curve -> p: Spec.ECC.point #c -> Lemma 
+  (isPointAtInfinity #c #Jacobian p == isPointAtInfinity #c #Jacobian (fromDomainPoint #c #DH p))
+
+let lemma_pointAtInfInDomain1 #c p = 
+  let (x, y, z) = p in 
+  lemma_pointAtInfInDomain #c x y z
+
+
+inline_for_extraction noextract
+val generatePrecomputedTable_0: #c: curve -> precomputedTable: lbuffer uint64 (getPointLenU64 c *! 16ul) 
+  -> publicKey: point c -> 
+  Stack unit  
+  (requires fun h -> live h precomputedTable /\ live h publicKey /\ point_eval c h publicKey /\ 
+    disjoint publicKey precomputedTable /\ 
+    ~ (isPointAtInfinity #c (fromDomainPoint #c #DH (point_as_nat c h publicKey))))
+  (ensures fun h0 _ h1 -> modifies (loc precomputedTable) h0 h1 /\ (
+    forall (i: nat {i < 2}). let pi = getPointTable c precomputedTable i in point_eval c h1 pi) /\ (
+    forall (i: nat {i < 2}). 
+      let pi = fromDomainPoint #c #DH (point_as_nat c h1 (getPointTable c precomputedTable i)) in 
+      let p1 = fromDomainPoint #c #DH (point_as_nat c h1 (getPointTable c precomputedTable 1)) in 
+      let p  = fromDomainPoint #c #DH (point_as_nat c h0 publicKey) in
+      ~ (isPointAtInfinity #c p1) /\ (exists (z: nat {z <= getOrder #c / 16}). pointEqual p (point_mult #c z p1)) /\ 
+	pointEqual pi (point_mult #c i p1)))
+
+let generatePrecomputedTable_0 #c table publicKey = 
+  let pointLen = getPointLenU64 c in 
+  let point0 = sub table (size 0) pointLen in 
+  let point1 = sub table pointLen pointLen in 
+
+  let h0 = ST.get() in 
+  Hacl.Impl.EC.LowLevel.uploadZeroPoint #c point0;
+  let h1 = ST.get() in 
+  Hacl.Impl.EC.LowLevel.copy_point #c publicKey point1;
+  let h2 = ST.get() in 
+
+  assert(getPointTable c table 0 == gsub table (pointLen *! size 0) pointLen);
+  assert(getPointTable c table 1 == gsub table (pointLen *! size 1) pointLen);
+
+  let p1 = fromDomainPoint #c #DH (point_as_nat c h2 (getPointTable c table 1)) in 
+  let p  = fromDomainPoint #c #DH (point_as_nat c h0 publicKey) in
+
+  point_mult_0 #c p1 0; 
+  lemma_pointAtInfInDomain1 #c (point_as_nat c h1 (getPointTable c table 0));
+  point_mult_1 #c p1
+
+
+val getPointTableLemma: #c: curve -> table: lbuffer uint64 (getPointLenU64 c *! 16ul) -> i: size_t {v i < 16} -> Lemma 
+  (getPointTable c table (v i) == gsub table (getPointLenU64 c *! i) (getPointLenU64 c))
+
+let getPointTableLemma #c table i = ()
+
+
+val lemma_getPointTable0: #c: curve -> i: size_t {v i >= 1 /\ v i <= 7} -> h: mem
+  -> table: lbuffer uint64 (getPointLenU64 c *! 16ul) -> 
+  Lemma
+  (requires (forall (j: nat {j < 2 * v i}). let pi = getPointTable c table j in point_eval c h pi))
+  (ensures (
+    let pointLen = getPointLenU64 c in 
+  
+    let point1 = gsub table pointLen pointLen in 
+    let point_n = gsub table (i *! pointLen) pointLen in 
+    let point_2n = gsub table (2ul *! i *! pointLen) pointLen in 
+    let point_2n_1 = gsub table ((2ul *! i +! 1ul) *! pointLen) pointLen in 
     
-  assume(invK h0 0);
+    disjoint point_n point_2n /\ point_eval c h point_n /\ point_eval c h point1 ))
+    
 
-  Lib.Loops.for (size 0) (size 16) invK f;
+let lemma_getPointTable0 #c i h table = 
+  let pointLen = getPointLenU64 c in 
+  
+  let point1 = gsub table pointLen pointLen in 
+  let point_n = gsub table (i *! pointLen) pointLen in 
+  let point_2n = gsub table (2ul *! i *! pointLen) pointLen in 
+  let point_2n_1 = gsub table ((2ul *! i +! 1ul) *! pointLen) pointLen in 
+    
+  assert(disjoint point_n point_2n);
+  getPointTableLemma #c table i;
+  getPointTableLemma #c table (size 1); 
+  
+  assert(getPointTable c table 1 == gsub table (pointLen *! (size 1)) (getPointLenU64 c));
 
-  admit()
+  assert(getPointTable c table (v i) == gsub table (getPointLenU64 c *! size (v i)) (getPointLenU64 c));
+  assert(getPointTable c table (v i) == gsub table (i *! pointLen) pointLen)
 
 
+val lemma_getPointTable1: #c: curve -> i: size_t {v i >= 1 /\ v i <= 7} -> h0: mem -> h1: mem 
+  -> table: lbuffer uint64 (getPointLenU64 c *! 16ul) -> tempBuffer: lbuffer uint64 (size 17 *! getCoordinateLenU64 c) ->
+  Lemma
+  (requires (
+    let pointLen = getPointLenU64 c in 
+    let point_2n = gsub table (2ul *! i *! pointLen) pointLen in 
+    modifies (loc point_2n |+| loc tempBuffer) h0 h1 /\ disjoint table tempBuffer /\ live h0 table /\ (
+    forall (j: nat {j < 2 * v i}). let pi = getPointTable c table j in point_eval c h0 pi)))
+  (ensures (
+    let pointLen = getPointLenU64 c in 
+  
+    let point1 = gsub table pointLen pointLen in 
+    let point_n = gsub table (i *! pointLen) pointLen in 
+    let point_2n = gsub table (2ul *! i *! pointLen) pointLen in 
+    let point_2n_1 = gsub table ((2ul *! i +! 1ul) *! pointLen) pointLen in 
+    
+    eq_or_disjoint point1 point_2n_1 /\ disjoint point_2n point1 /\ disjoint point_2n point_2n_1 /\ point_eval c h1 point1))
 
+let lemma_getPointTable1 #c i h0 h1 table tempBuffer = 
+  let pointLen = getPointLenU64 c in 
+  
+  let point1 = gsub table pointLen pointLen in 
+  let point_n = gsub table (i *! pointLen) pointLen in 
+  let point_2n = gsub table (2ul *! i *! pointLen) pointLen in 
+  let point_2n_1 = gsub table ((2ul *! i +! 1ul) *! pointLen) pointLen in 
+
+  getPointTableLemma table (size 1); 
+  assert(getPointTable c table 1 == gsub table (pointLen *! size 1) (pointLen));
+
+  Hacl.Impl.P.PointAdd.Aux.lemma_coord_eval c h0 h1 point1
+
+
+val lemma_getPointTable2_0: #c: curve -> i: size_t {v i >= 1 /\ v i <= 7} -> h0: mem -> h1: mem 
+  -> table: lbuffer uint64 (getPointLenU64 c *! 16ul) -> tempBuffer: lbuffer uint64 (size 17 *! getCoordinateLenU64 c) ->
+  Lemma (requires (
+    live h0 table /\ live h0 tempBuffer /\ disjoint table tempBuffer /\ (
+      let pointLen = getPointLenU64 c in 
+      let point_2n = gsub table (2ul *! i *! pointLen) pointLen in 
+      let point_2n_1 = gsub table ((2ul *! i +! 1ul) *! pointLen) pointLen in 
+      modifies (loc point_2n |+| loc point_2n_1 |+| loc tempBuffer) h0 h1)))
+  (ensures (
+    let pointLen = getPointLenU64 c in 
+    let allPointsBefore = gsub table (size 0) (2ul *! i *! pointLen) in 
+    as_seq h0 allPointsBefore == as_seq h1 allPointsBefore))
+
+let lemma_getPointTable2_0 #c i h0 h1 table tempBuffer = 
+  let pointLen = getPointLenU64 c in 
+  let allPointsBefore = gsub table (size 0) (2ul *! i *! pointLen) in 
+  
+  let point_2n = gsub table (2ul *! i *! pointLen) pointLen in 
+  let point_2n_1 = gsub table ((2ul *! i +! 1ul) *! pointLen) pointLen in 
+  assert(as_seq h0 allPointsBefore == as_seq h1 allPointsBefore)
+
+
+val lemma_getPointTable2_1_0: #c: curve -> i: size_t {v i >= 1 /\ v i <= 7} -> h0: mem -> h1: mem 
+  -> table: lbuffer uint64 (getPointLenU64 c *! 16ul) -> k: nat {k < 2 * v i} ->
+  Lemma 
+  (requires (
+    let pointLen = getPointLenU64 c in 
+    let allPointsBefore = gsub table (size 0) (2ul *! i *! pointLen) in 
+    as_seq h0 allPointsBefore == as_seq h1 allPointsBefore /\ 
+    point_eval c h0 (getPointTable c table k)))
+  (ensures (point_eval c h1 (getPointTable c table k)))
+
+let lemma_getPointTable2_1_0 #c i h0 h1 table k = 
+  let pointLen = getPointLenU64 c in 
+  let allPointsBefore = gsub table (size 0) (2ul *! i *! pointLen) in 
+  let pk = gsub table (size k *! getPointLenU64 c) (getPointLenU64 c) in 
+  
+  assert(gsub table (size k *! getPointLenU64 c) (getPointLenU64 c) == gsub allPointsBefore (size k *! getPointLenU64 c) (getPointLenU64 c));
+  assert (getZ pk == gsub pk (size 2 *! (getCoordinateLenU64 c)) (getCoordinateLenU64 c))
+
+ 
+val lemma_getPointTable2_1: #c: curve -> i: size_t {v i >= 1 /\ v i <= 7} -> h0: mem -> h1: mem 
+  -> table: lbuffer uint64 (getPointLenU64 c *! 16ul) -> 
+  Lemma 
+  (requires (
+    let pointLen = getPointLenU64 c in 
+    let allPointsBefore = gsub table (size 0) (2ul *! i *! pointLen) in 
+    as_seq h0 allPointsBefore == as_seq h1 allPointsBefore /\ 
+    (forall (k: nat {k < 2 * v i}). point_eval c h0 (getPointTable c table k))))
+  (ensures (forall (k: nat {k < 2 * v i}). 
+    point_eval c h1 (getPointTable c table k)))
+
+let lemma_getPointTable2_1 #c i h0 h1 table = 
+  let a: Type = a: nat {a < 2 * v i} in 
+  let p : (a -> GTot Type) = 
+    fun i -> point_eval c h1 (getPointTable c table i) in 
+  let pred : (x : a -> Lemma (p x)) = lemma_getPointTable2_1_0 #c i h0 h1 table in 
+  Classical.forall_intro #a #p pred
+  
+
+val getPointTableLemma_1: #c: curve -> table: lbuffer uint64 (getPointLenU64 c *! 16ul) -> Lemma
+    (getPointTable c table 1 == gsub table (getPointLenU64 c) (getPointLenU64 c))
+
+let getPointTableLemma_1 #c table = ()
+
+
+val lemma_getPointTable2_2: #c: curve -> i: size_t {v i >= 1 /\ v i <= 7} -> h0: mem -> h1: mem 
+  -> table: lbuffer uint64 (getPointLenU64 c *! 16ul) {live h0 table} ->
+  Lemma 
+  (requires (
+    let pointLen = getPointLenU64 c in 
+    let allPointsBefore = gsub table (size 0) (2ul *! i *! pointLen) in 
+    as_seq h0 allPointsBefore == as_seq h1 allPointsBefore /\ (
+    point_eval c h0 (getPointTable c table 1) /\ (
+    let p1 = fromDomainPoint #c #DH (point_as_nat c h0 (getPointTable c table 1)) in 
+    ~ (isPointAtInfinity #c p1)))))
+  (ensures (
+    point_eval c h1 (getPointTable c table 1) /\ (
+    let p1 = fromDomainPoint #c #DH (point_as_nat c h1 (getPointTable c table 1)) in 
+    ~ (isPointAtInfinity #c p1))))
+
+let lemma_getPointTable2_2 #c i h0 h1 table = 
+  let pointLen = getPointLenU64 c in 
+  let allPointsBefore = gsub table (size 0) (2ul *! i *! pointLen) in 
+  let point1 = gsub table pointLen pointLen in 
+
+  getPointTableLemma_1 table; 
+  assert (gsub table pointLen pointLen == gsub allPointsBefore pointLen pointLen); 
+  assert (getZ point1 == gsub point1 (size 2 *! (getCoordinateLenU64 c)) (getCoordinateLenU64 c))
+
+
+val lemma_getPointTable2: #c: curve -> i: size_t {v i >= 1 /\ v i <= 7} -> h0: mem -> h1: mem 
+  -> table: lbuffer uint64 (getPointLenU64 c *! 16ul) -> tempBuffer: lbuffer uint64 (size 17 *! getCoordinateLenU64 c) ->
+  Lemma (requires (
+    live h0 table /\ live h0 tempBuffer /\ disjoint table tempBuffer /\ (
+      let pointLen = getPointLenU64 c in 
+      let point_2n = gsub table (2ul *! i *! pointLen) pointLen in 
+      let point_2n_1 = gsub table ((2ul *! i +! 1ul) *! pointLen) pointLen in 
+      modifies (loc point_2n |+| loc point_2n_1 |+| loc tempBuffer) h0 h1 /\ 
+      point_eval c h1 point_2n /\ point_eval c h1 point_2n_1 /\ (
+      forall (j: nat {j < 2 * v i}). let pi = getPointTable c table j in point_eval c h0 pi) /\ (
+      forall (j: nat {j < 2 * v i}).
+	let pi = fromDomainPoint #c #DH (point_as_nat c h0 (getPointTable c table j)) in 
+	let p1 = fromDomainPoint #c #DH (point_as_nat c h0 (getPointTable c table 1)) in 
+	~ (isPointAtInfinity #c p1) /\ pointEqual pi (point_mult #c j p1)))))
+  (ensures (
+      forall (j: nat {j <= 2 * v i + 1}). let pi = getPointTable c table j in point_eval c h1 pi) /\ (
+      forall (j: nat {j <= 2 * v i + 1}). 
+      let pi = fromDomainPoint #c #DH (point_as_nat c h1 (getPointTable c table j)) in 
+      let p1 = fromDomainPoint #c #DH (point_as_nat c h1 (getPointTable c table 1)) in 
+      ~ (isPointAtInfinity #c p1 /\ pointEqual pi (point_mult #c j p1))))
+
+let lemma_getPointTable2 #c i h0 h1 table tempBuffer = 
+  lemma_getPointTable2_0 i h0 h1 table tempBuffer;
+  lemma_getPointTable2_1 #c i h0 h1 table;
+
+  getPointTableLemma table (2ul *! i);
+  getPointTableLemma table (2ul *! i +! 1ul);
+
+  lemma_getPointTable2_2 i h0 h1 table
+  
+
+val generatePrecomputedTable_1: #c: curve -> precomputedTable: lbuffer uint64 (getPointLenU64 c *! 16ul) 
+  -> i: size_t {v i >= 1 /\ v i <= 7}
+  -> tempBuffer: lbuffer uint64 (size 17 *! getCoordinateLenU64 c) ->
+  Stack unit  
+  (requires fun h -> live h precomputedTable /\ live h tempBuffer /\ disjoint precomputedTable tempBuffer /\ (
+    forall (j: nat {j < 2 * v i}). let pi = getPointTable c precomputedTable j in point_eval c h pi) /\ (
+    forall (j: nat {j < 2 * v i}). 
+      let pi = fromDomainPoint #c #DH (point_as_nat c h (getPointTable c precomputedTable j)) in 
+      let p1 = fromDomainPoint #c #DH (point_as_nat c h (getPointTable c precomputedTable 1)) in 
+      ~ (isPointAtInfinity #c p1) /\ pointEqual pi (point_mult #c j p1)))
+  (ensures fun h0 _ h1 -> modifies (loc precomputedTable |+| loc tempBuffer) h0 h1 /\ (
+    forall (j: nat {j <= 2 * v i + 1}). let pi = getPointTable c precomputedTable j in point_eval c h1 pi) /\ (
+    forall (j: nat {j <= 2 * v i + 1}). 
+      let pi = fromDomainPoint #c #DH (point_as_nat c h1 (getPointTable c precomputedTable j)) in 
+      let p1 = fromDomainPoint #c #DH (point_as_nat c h1 (getPointTable c precomputedTable 1)) in 
+      ~ (isPointAtInfinity #c p1 /\ pointEqual pi (point_mult #c j p1))))
+
+
+let generatePrecomputedTable_1 #c table i tempBuffer =
+  let pointLen = getPointLenU64 c in 
+  
+  let point1 = sub table pointLen pointLen in 
+  let point_n = sub table (i *! pointLen) pointLen in 
+  let point_2n = sub table (2ul *! i *! pointLen) pointLen in 
+  let point_2n_1 = sub table ((2ul *! i +! 1ul) *! pointLen) pointLen in 
+
+  let h0 = ST.get() in 
+
+  lemma_getPointTable0 #c i h0 table;
+  point_double #c point_n point_2n tempBuffer;
+  
+  let h1 = ST.get() in 
+
+  lemma_getPointTable1 i h0 h1 table tempBuffer;
+  point_add point_2n point1 point_2n_1 tempBuffer;
+
+  let h2 = ST.get() in 
+
+  Hacl.Impl.P.PointAdd.Aux.lemma_coord_eval c h1 h2 point_2n;
+  lemma_getPointTable2 i h0 h2 table tempBuffer
 
 (*
-inline_for_extraction noextract  
-val montgomery_ladder_step_radix: 
-   #c: curve ->
-  p: point P256 -> tempBuffer: lbuffer uint64 (size 88) -> 
-  precomputedTable: lbuffer uint64 (size 192) ->
-  scalar:  lbuffer uint8 (size 32) -> 
-  i:size_t{v i < 256} -> 
-  Stack unit
-  (requires fun h -> live h p /\live h tempBuffer /\ live h scalar /\
-    LowStar.Monotonic.Buffer.all_disjoint [loc p;loc tempBuffer; loc scalar])
-  (ensures fun h0 _ h1 -> True)
-
-
-let montgomery_ladder_step_radix #c p tempBuffer precomputedTable scalar i =  
-  let bits = getScalar_4_byBit #c scalar i in 
-
-  let pointToAdd = create (size 12) (u64 0) in 
-  getPointPrecomputedTable #c scalar precomputedTable i pointToAdd; 
-  
-  point_double p p tempBuffer;
-  point_double p p tempBuffer;
-  point_double p p tempBuffer;
-  point_double p p tempBuffer;
-
-  point_add pointToAdd p p tempBuffer
-
-
 [@ CInline]
-val generatePrecomputedTable: #c: curve -> b: lbuffer uint64 (size 192) -> publicKey: point c ->
-  tempBuffer: lbuffer uint64 (size 88) -> Stack unit  
+val generatePrecomputedTable: #c: curve -> precomputedTable: lbuffer uint64 (getPointLen c *! 16ul) 
+  -> publicKey: point c 
+  -> tempBuffer: lbuffer uint64 (size 17 *! getCoordinateLenU64 c) -> Stack unit  
   (requires fun h -> True)
   (ensures fun h0 _ h1 -> True)
 
 let generatePrecomputedTable #c b publicKey tempBuffer = 
-  let point0 = sub b (size 0) (size 12) in 
-  let point1 = sub b (size 12) (size 12) in 
-  let point2 = sub b (size 24) (size 12) in 
-  let point3 = sub b (size 36) (size 12) in 
-  let point4 = sub b (size 48) (size 12) in 
-  let point5 = sub b (size 60) (size 12) in 
-  let point6 = sub b (size 72) (size 12) in 
-  let point7 = sub b (size 84) (size 12) in 
-  let point8 = sub b (size 96) (size 12) in 
-  let point9 = sub b (size 108) (size 12) in 
-  let point10 = sub b (size 120) (size 12) in 
-  let point11 = sub b (size 132) (size 12) in 
-  let point12 = sub b (size 144) (size 12) in 
-  let point13 = sub b (size 156) (size 12) in 
-  let point14 = sub b (size 168) (size 12) in 
-  let point15 = sub b (size 180) (size 12) in 
+  generatePrecomputedTable_0 b publicKey;
 
-  Hacl.Impl.EC.LowLevel.uploadZeroPoint #c point0;
-  Hacl.Impl.EC.LowLevel.copy_point #c publicKey point1;
-  point_double #c publicKey point2 tempBuffer;
-  point_add #c point2 point1 point3 tempBuffer;
-  point_double #c point2 point4 tempBuffer;
-  point_add #c point4 point1 point5 tempBuffer;
-  point_double #c point3 point6 tempBuffer;
-  point_add #c point6 point1 point7 tempBuffer;
-  point_double #c point4 point8 tempBuffer;
-  point_add #c point8 point1 point9 tempBuffer;
-  point_double #c point5 point10 tempBuffer;
-  point_add #c point10 point1 point11 tempBuffer;
-  point_double #c point6 point12 tempBuffer;
-  point_add #c point12 point1 point13 tempBuffer;
-  point_double #c point7 point14 tempBuffer;
-  point_add #c point14 point1 point15 tempBuffer
+  generatePrecomputedTable_1 b (size 1) tempBuffer;
+  generatePrecomputedTable_1 b (size 2) tempBuffer;
+  generatePrecomputedTable_1 b (size 3) tempBuffer;
+  generatePrecomputedTable_1 b (size 4) tempBuffer;
+  generatePrecomputedTable_1 b (size 5) tempBuffer;
+  generatePrecomputedTable_1 b (size 6) tempBuffer;
+  generatePrecomputedTable_1 b (size 7) tempBuffer
 
 
 
@@ -701,26 +1065,25 @@ val montgomery_ladder_2: #buf_type: buftype -> #c: curve -> p: point c ->
 
 let montgomery_ladder_2 #a #c p scalar tempBuffer precomputedTable =  
  let h0 = ST.get() in 
-   push_frame();
+ push_frame();
 
-     [@inline_let]
-     let spec_ml h0 = _ml_step #c (as_seq h0 scalar) in 
+ [@inline_let]
+ let spec_ml h0 = _ml_step #c (as_seq h0 scalar) in 
+ [@inline_let]
+ let inv h (i: nat {i <= 64}) = True in 
 
-
-     [@inline_let]
-     let inv h (i: nat {i <= 64}) = True in 
-
+   let pointLen = getPointLenU64 c in 
 
   let bits =  getScalar_4_byBit #c  scalar (u64 0) in 
-  let pointToStart = sub precomputedTable  (bits *. size 12) (size 12) in 
+  let pointToStart = sub precomputedTable  (bits *. pointLen) pointLen in 
+  copy (sub p (size 0) pointLen) pointToStart;
 
-  copy (sub p (size 0) (size 12)) pointToStart;
-  
-     for 1ul 64ul inv 
-       (fun i -> let h2 = ST.get() in
-   montgomery_ladder_step_radix #c p tempBuffer precomputedTable scalar i
-       );
-   pop_frame()
+ let r = create (size 3 *! getCoordinateLenU64 c) (u64 0) in 
+ for 1ul (size 2 *! getScalarLenBytes c)  inv 
+   (fun i -> let h2 = ST.get() in
+   montgomery_ladder_step_radix #c #a p scalar precomputedTable i tempBuffer r);
+ 
+ pop_frame()
 
 
 
@@ -748,7 +1111,7 @@ let scalar_multiplication_t_0 #c p result scalar tempBuffer =
   uploadStartPoints q p result; 
   montgomery_ladder q result scalar tempBuffer;
   copy q result *)
-  let bufferPrecomputed = create (size 192) (u64 0) in 
+  let bufferPrecomputed = create (size 16 *! getPointLen c) (u64 0) in 
   generatePrecomputedTable bufferPrecomputed result tempBuffer;
   montgomery_ladder_2 result scalar tempBuffer bufferPrecomputed
 
