code/ecdsa/Hacl.Impl.EC.PointAdd.fsti
@@ -25,7 +25,10 @@ val point_add: #c: curve -> p: point c -> q: point c -> result: point c
     eq_or_disjoint q result /\ disjoint p q /\ disjoint p tempBuffer /\ 
     disjoint q tempBuffer /\ disjoint p result /\ disjoint result tempBuffer /\  
     point_eval c h p /\ point_eval c h q)
-  (ensures fun h0 _ h1 -> modifies (loc tempBuffer |+| loc result) h0 h1)
+  (ensures fun h0 _ h1 -> modifies (loc tempBuffer |+| loc result) h0 h1 /\ point_eval c h1 result /\ 
+    fromDomainPoint #c #DH (point_as_nat c h1 result) == 
+      _point_add #c (fromDomainPoint #c #DH (point_as_nat c h0 p)) 
+        (fromDomainPoint #c #DH (point_as_nat c h0 q)))
 
   
 inline_for_extraction noextract
